backends/lean/Base/Progress/Progress.lean
@@ -39,7 +39,7 @@ inductive ProgressError
 | Error (msg : MessageData)
 deriving Inhabited
 
-def progressWith (fnExpr : Expr) (th : TheoremOrLocal) (ids : Array Name)
+def progressWith (fnExpr : Expr) (th : TheoremOrLocal) (keep : Option Name) (ids : Array Name)
   (asmTac : TacticM Unit) : TacticM ProgressError := do
   /- Apply the theorem
      We try to match the theorem with the goal
@@ -88,7 +88,7 @@ def progressWith (fnExpr : Expr) (th : TheoremOrLocal) (ids : Array Name)
     match th with
     | .Theorem thName => mkAppOptM thName (mvars.map some)
     | .Local decl => mkAppOptM' (mkFVar decl.fvarId) (mvars.map some)
-  let asmName ← mkFreshUserName `h
+  let asmName ← do match keep with | none => mkFreshUserName `h | some n => do pure n
   let thTy ← inferType th
   let thAsm ← Utils.addDeclTac asmName th thTy (asLet := false)
   withMainContext do -- The context changed - TODO: remove once addDeclTac is updated
@@ -109,7 +109,9 @@ def progressWith (fnExpr : Expr) (th : TheoremOrLocal) (ids : Array Name)
       if ← isConj (← inferType h) then do
         let hName := (← h.fvarId!.getDecl).userName
         let (optId, ids) := listTryPopHead ids
-        let optIds := match optId with | none => none | some id => some (hName, id)
+        let optIds ← match optId with
+          | none => do pure (some (hName, ← mkFreshUserName `h))
+          | some id => do pure (some (hName, id))
         splitConjTac h optIds (fun hEq hPost => k hEq (some hPost) ids)
       else k h none ids
     -- Simplify the target by using the equality and some monad simplifications,
@@ -118,9 +120,12 @@ def progressWith (fnExpr : Expr) (th : TheoremOrLocal) (ids : Array Name)
     trace[Progress] "eq and post:\n{hEq} : {← inferType hEq}\n{hPost}"
     simpAt [] [``Primitives.bind_tc_ret, ``Primitives.bind_tc_fail, ``Primitives.bind_tc_div]
            [hEq.fvarId!] (.targets #[] true)
-    -- Clear the equality
-    let mgoal ← getMainGoal
-    let mgoal ← mgoal.tryClearMany #[hEq.fvarId!]
+    -- Clear the equality, unless the user requests not to do so
+    let mgoal ← do
+      if keep.isSome then getMainGoal
+      else do
+        let mgoal ← getMainGoal
+        mgoal.tryClearMany #[hEq.fvarId!]
     setGoals (mgoal :: (← getUnsolvedGoals))
     trace[Progress] "Goal after splitting eq and post and simplifying the target: {mgoal}"
     -- Continue splitting following the ids provided by the user
@@ -170,7 +175,7 @@ def getFirstArg (args : Array Expr) : Option Expr := do
 
 /- Helper: try to lookup a theorem and apply it, or continue with another tactic
    if it fails -/
-def tryLookupApply (ids : Array Name) (asmTac : TacticM Unit) (fnExpr : Expr)
+def tryLookupApply (keep : Option Name) (ids : Array Name) (asmTac : TacticM Unit) (fnExpr : Expr)
   (kind : String) (th : Option TheoremOrLocal) (x : TacticM Unit) : TacticM Unit := do
   let res ← do
     match th with
@@ -182,7 +187,7 @@ def tryLookupApply (ids : Array Name) (asmTac : TacticM Unit) (fnExpr : Expr)
       -- Apply the theorem
       let res ← do
         try
-          let res ← progressWith fnExpr th ids asmTac
+          let res ← progressWith fnExpr th keep ids asmTac
           pure (some res)
         catch _ => none
   match res with
@@ -191,7 +196,7 @@ def tryLookupApply (ids : Array Name) (asmTac : TacticM Unit) (fnExpr : Expr)
   | none => x
 
 -- The array of ids are identifiers to use when introducing fresh variables
-def progressAsmsOrLookupTheorem (withTh : Option TheoremOrLocal) (ids : Array Name) (asmTac : TacticM Unit) : TacticM Unit := do
+def progressAsmsOrLookupTheorem (keep : Option Name) (withTh : Option TheoremOrLocal) (ids : Array Name) (asmTac : TacticM Unit) : TacticM Unit := do
   withMainContext do
   -- Retrieve the goal
   let mgoal ← Tactic.getMainGoal
@@ -209,7 +214,7 @@ def progressAsmsOrLookupTheorem (withTh : Option TheoremOrLocal) (ids : Array Na
   -- Otherwise, lookup one.
   match withTh with
   | some th => do
-    match ← progressWith fnExpr th ids asmTac with
+    match ← progressWith fnExpr th keep ids asmTac with
     | .Ok => return ()
     | .Error msg => throwError msg
   | none =>
@@ -218,7 +223,7 @@ def progressAsmsOrLookupTheorem (withTh : Option TheoremOrLocal) (ids : Array Na
     let decls ← ctx.getDecls
     for decl in decls.reverse do
       trace[Progress] "Trying assumption: {decl.userName} : {decl.type}"
-      let res ← do try progressWith fnExpr (.Local decl) ids asmTac catch _ => continue
+      let res ← do try progressWith fnExpr (.Local decl) keep ids asmTac catch _ => continue
       match res with
       | .Ok => return ()
       | .Error msg => throwError msg
@@ -228,7 +233,7 @@ def progressAsmsOrLookupTheorem (withTh : Option TheoremOrLocal) (ids : Array Na
     let pspec ← do
       let thName ← pspecAttr.find? fName
       pure (thName.map fun th => .Theorem th)
-    tryLookupApply ids asmTac fnExpr "pspec theorem" pspec do
+    tryLookupApply keep ids asmTac fnExpr "pspec theorem" pspec do
     -- It failed: try to lookup a *class* expr spec theorem (those are more
     -- specific than class spec theorems)
     let pspecClassExpr ← do
@@ -237,7 +242,7 @@ def progressAsmsOrLookupTheorem (withTh : Option TheoremOrLocal) (ids : Array Na
       | some arg => do
         let thName ← pspecClassExprAttr.find? fName arg
         pure (thName.map fun th => .Theorem th)
-    tryLookupApply ids asmTac fnExpr "pspec class expr theorem" pspecClassExpr do
+    tryLookupApply keep ids asmTac fnExpr "pspec class expr theorem" pspecClassExpr do
     -- It failed: try to lookup a *class* spec theorem
     let pspecClass ← do
       match ← getFirstArgAppName args with
@@ -245,7 +250,7 @@ def progressAsmsOrLookupTheorem (withTh : Option TheoremOrLocal) (ids : Array Na
       | some argName => do
         let thName ← pspecClassAttr.find? fName argName
         pure (thName.map fun th => .Theorem th)
-    tryLookupApply ids asmTac fnExpr "pspec class theorem" pspecClass do
+    tryLookupApply keep ids asmTac fnExpr "pspec class theorem" pspecClass do
     -- Try a recursive call - we try the assumptions of kind "auxDecl"
     let ctx ← Lean.MonadLCtx.getLCtx
     let decls ← ctx.getAllDecls
@@ -253,21 +258,29 @@ def progressAsmsOrLookupTheorem (withTh : Option TheoremOrLocal) (ids : Array Na
       | .default | .implDetail => false | .auxDecl => true)
     for decl in decls.reverse do
       trace[Progress] "Trying recursive assumption: {decl.userName} : {decl.type}"
-      let res ← do try progressWith fnExpr (.Local decl) ids asmTac catch _ => continue
+      let res ← do try progressWith fnExpr (.Local decl) keep ids asmTac catch _ => continue
       match res with
       | .Ok => return ()
       | .Error msg => throwError msg
     -- Nothing worked: failed
     throwError "Progress failed"
 
-syntax progressArgs := ("with" ident)? ("as" " ⟨ " (ident)+ " ⟩")?
+syntax progressArgs := ("keep" ("as" (ident))?)? ("with" ident)? ("as" " ⟨ " (ident)+ " ⟩")?
 
 def evalProgress (args : TSyntax `Progress.progressArgs) : TacticM Unit := do
   let args := args.raw
   -- Process the arguments to retrieve the identifiers to use
   trace[Progress] "Progress arguments: {args}"
   let args := args.getArgs
-  let withArg := (args.get! 0).getArgs
+  let keep : Option Name ← do
+    let args := (args.get! 0).getArgs
+    if args.size > 0 then do
+      let args := (args.get! 1).getArgs
+      if args.size > 0 then pure (some (args.get! 1).getId)
+      else do pure (some (← mkFreshUserName `h))
+    else pure none
+  trace[Progress] "Keep: {keep}"
+  let withArg := (args.get! 1).getArgs
   let withArg ← do
     if withArg.size > 0 then
       let id := withArg.get! 1
@@ -287,11 +300,11 @@ def evalProgress (args : TSyntax `Progress.progressArgs) : TacticM Unit := do
         | id :: _ =>
           pure (some (.Theorem id))
     else pure none
-  let args := (args.get! 1).getArgs
+  let args := (args.get! 2).getArgs
   let args := (args.get! 2).getArgs
   let ids := args.map Syntax.getId
   trace[Progress] "User-provided ids: {ids}"
-  progressAsmsOrLookupTheorem withArg ids (firstTac [assumptionTac, Arith.scalarTac])
+  progressAsmsOrLookupTheorem keep withArg ids (firstTac [assumptionTac, Arith.scalarTac])
 
 elab "progress" args:progressArgs : tactic =>
   evalProgress args
@@ -306,11 +319,11 @@ namespace Test
   #eval showStoredPSpec
   #eval showStoredPSpecClass
 
-  theorem Scalar.add_spec {ty} {x y : Scalar ty}
+  theorem Scalar.add_spec1 {ty} {x y : Scalar ty}
     (hmin : Scalar.min ty ≤ x.val + y.val)
     (hmax : x.val + y.val ≤ Scalar.max ty) :
     ∃ z, x + y = ret z ∧ z.val = x.val + y.val := by
-    progress
+    progress keep as h with Scalar.add_spec as ⟨ z ⟩
     simp [*]
 
 /-
